reflection/tactics: Introduce V2

ocaml/fstar-lib/FStar_Reflection_Types.ml
@@ -2,6 +2,7 @@ open FStar_All
 
 type binder  = FStar_Syntax_Syntax.binder
 type bv      = FStar_Syntax_Syntax.bv
+type namedv  = bv
 type term    = FStar_Syntax_Syntax.term
 type env     = FStar_TypeChecker_Env.env
 type fv      = FStar_Syntax_Syntax.fv
@@ -15,7 +16,7 @@ type universe_uvar = FStar_Syntax_Syntax.universe_uvar
 type universe = FStar_Syntax_Syntax.universe
 
 type name        = string list
-type ident       = string * FStar_Compiler_Range.range
+type ident       = FStar_Ident.ident
 type univ_name   = ident
 type typ         = term
 type binders     = binder list
