src/reflection/FStar.Reflection.V2.Interpreter.fst
@@ -1,0 +1,458 @@
+(*
+   Copyright 2008-2022 Microsoft Research
+
+   Licensed under the Apache License, Version 2.0 (the "License");
+   you may not use this file except in compliance with the License.
+   You may obtain a copy of the License at
+
+       http://www.apache.org/licenses/LICENSE-2.0
+
+   Unless required by applicable law or agreed to in writing, software
+   distributed under the License is distributed on an "AS IS" BASIS,
+   WITHOUT WARRANTIES OR CONDITIONS OF ANY KIND, either express or implied.
+   See the License for the specific language governing permissions and
+   limitations under the License.
+*)
+module FStar.Reflection.V2.Interpreter
+
+module BU    = FStar.Compiler.Util
+module Cfg   = FStar.TypeChecker.Cfg
+module EMB   = FStar.Syntax.Embeddings
+module Env   = FStar.TypeChecker.Env
+module NBET  = FStar.TypeChecker.NBETerm
+module NRE   = FStar.Reflection.V2.NBEEmbeddings
+module RB    = FStar.Reflection.V2.Builtins
+module RD    = FStar.Reflection.V2.Data
+module RE    = FStar.Reflection.V2.Embeddings
+module Z     = FStar.BigInt
+module Range = FStar.Compiler.Range
+open FStar.Compiler
+open FStar.Compiler.List
+open FStar.Ident
+open FStar.Syntax.Syntax
+open FStar.Reflection.V2.Constants
+
+let unembed      = EMB.unembed
+let try_unembed  = EMB.try_unembed
+let embed ea r x norm_cb     = EMB.embed ea x r None norm_cb
+
+(* We use `try_unembed` instead of `unembedding`, since we very well
+ * might fail to unembed during the *previous* normalization stages
+ * of metaprograms. When actually running, we certainly expect
+ * everything to reduce to proper values and unembed just fine, but
+ * we cannot ignore this case. So, use `try_` so we don't generate
+ * spurious warnings. *)
+
+let int1 (m:lid) (f:'a -> 'r) (ea:EMB.embedding 'a) (er:EMB.embedding 'r)
+                 (psc:Cfg.psc) n (args : args) : option term =
+    match args with
+    | [(a, _)] ->
+        BU.bind_opt (try_unembed ea a n) (fun a ->
+        Some (embed er (Cfg.psc_range psc) (f a) n))
+    | _ -> None
+
+let int2 (m:lid) (f:'a -> 'b -> 'r) (ea:EMB.embedding 'a) (eb:EMB.embedding 'b) (er:EMB.embedding 'r)
+                 (psc:Cfg.psc) n (args : args) : option term =
+    match args with
+    | [(a, _); (b, _)] ->
+        BU.bind_opt (try_unembed ea a n) (fun a ->
+        BU.bind_opt (try_unembed eb b n) (fun b ->
+        Some (embed er (Cfg.psc_range psc) (f a b) n)))
+    | _ -> None
+
+let int3 (m:lid) (f:'a -> 'b -> 'c -> 'r) (ea:EMB.embedding 'a) (eb:EMB.embedding 'b) (ec:EMB.embedding 'c) (er:EMB.embedding 'r)
+                 (psc:Cfg.psc) n (args : args) : option term =
+    match args with
+    | [(a, _); (b, _); (c, _)] ->
+        BU.bind_opt (try_unembed ea a n) (fun a ->
+        BU.bind_opt (try_unembed eb b n) (fun b ->
+        BU.bind_opt (try_unembed ec c n) (fun c ->
+        Some (embed er (Cfg.psc_range psc) (f a b c) n))))
+    | _ -> None
+
+let nbe_int1 (m:lid) (f:'a -> 'r) (ea:NBET.embedding 'a) (er:NBET.embedding 'r)
+                     (cb:NBET.nbe_cbs) (args : NBET.args) : option NBET.t =
+    match args with
+    | [(a, _)] ->
+        BU.bind_opt (NBET.unembed ea cb a) (fun a ->
+        Some (NBET.embed er cb (f a)))
+    | _ -> None
+
+let nbe_int2 (m:lid) (f:'a -> 'b -> 'r) (ea:NBET.embedding 'a) (eb:NBET.embedding 'b) (er:NBET.embedding 'r)
+                     (cb:NBET.nbe_cbs) (args : NBET.args) : option NBET.t =
+    match args with
+    | [(a, _); (b, _)] ->
+        BU.bind_opt (NBET.unembed ea cb a) (fun a ->
+        BU.bind_opt (NBET.unembed eb cb b) (fun b ->
+        Some (NBET.embed er cb (f a b))))
+    | _ -> None
+
+let nbe_int3 (m:lid) (f:'a -> 'b -> 'c -> 'r) (ea:NBET.embedding 'a) (eb:NBET.embedding 'b) (ec:NBET.embedding 'c) (er:NBET.embedding 'r)
+                     (cb:NBET.nbe_cbs) (args : NBET.args) : option NBET.t =
+    match args with
+    | [(a, _); (b, _); (c, _)] ->
+        BU.bind_opt (NBET.unembed ea cb a) (fun a ->
+        BU.bind_opt (NBET.unembed eb cb b) (fun b ->
+        BU.bind_opt (NBET.unembed ec cb c) (fun c ->
+        Some (NBET.embed er cb (f a b c)))))
+    | _ -> None
+
+let mklid (nm : string) : lid = fstar_refl_builtins_lid nm
+
+let mk_us (l : lid) (u_arity:int) (arity : int)
+            (fn     : Cfg.psc -> EMB.norm_cb -> args -> option term)
+            (nbe_fn : NBET.nbe_cbs -> NBET.args -> option NBET.t) : Cfg.primitive_step
+  =
+  { Cfg.name                         = l
+  ; Cfg.arity                        = arity
+  ; Cfg.univ_arity                   = u_arity
+  ; Cfg.auto_reflect                 = None
+  ; Cfg.strong_reduction_ok          = true
+  ; Cfg.requires_binder_substitution = false
+  ; Cfg.interpretation               = (fun psc cbs _us args -> fn psc cbs args)
+  ; Cfg.interpretation_nbe           = (fun cbs _us args -> nbe_fn cbs args)
+  }
+
+(* Most primitives are not universe polymorphic. *)
+let mk l arity fn nbe_fn = mk_us l 0 arity fn nbe_fn
+
+(*
+ ** Packing both regular and NBE embedding in a single type, for brevity
+ ** in the table below. This should all be unfolded at F* initialization
+ ** time so it won't be a performance concern.
+ *)
+type dualemb 'a = (EMB.embedding 'a & NBET.embedding 'a)
+
+let e_int             : dualemb Z.t                = (EMB.e_int, NBET.e_int)
+let e_bool            : dualemb bool               = (EMB.e_bool, NBET.e_bool)
+let e_string          : dualemb string             = (EMB.e_string, NBET.e_string)
+let e_order           : dualemb Order.order        = (RE.e_order, NRE.e_order)
+
+let e_term            : dualemb term               = (RE.e_term, NRE.e_term)
+let e_term_view       : dualemb RD.term_view       = (RE.e_term_view, NRE.e_term_view)
+let e_fv              : dualemb fv                 = (RE.e_fv, NRE.e_fv)
+let e_bv              : dualemb bv                 = (RE.e_bv, NRE.e_bv)
+let e_namedv          : dualemb RE.namedv          = (RE.e_namedv, NRE.e_namedv)
+let e_bv_view         : dualemb RD.bv_view         = (RE.e_bv_view, NRE.e_bv_view)
+let e_namedv_view     : dualemb RD.namedv_view     = (RE.e_namedv_view, NRE.e_namedv_view)
+let e_binding         : dualemb RD.binding         = (RE.e_binding, NRE.e_binding)
+let e_comp            : dualemb comp               = (RE.e_comp, NRE.e_comp)
+let e_comp_view       : dualemb RD.comp_view       = (RE.e_comp_view, NRE.e_comp_view)
+let e_universe        : dualemb universe           = (RE.e_universe, NRE.e_universe)
+let e_universe_view   : dualemb RD.universe_view   = (RE.e_universe_view, NRE.e_universe_view)
+let e_sigelt          : dualemb sigelt             = (RE.e_sigelt, NRE.e_sigelt)
+let e_sigelt_view     : dualemb RD.sigelt_view     = (RE.e_sigelt_view, NRE.e_sigelt_view)
+let e_binder          : dualemb binder             = (RE.e_binder, NRE.e_binder)
+let e_binder_view     : dualemb RD.binder_view     = (RE.e_binder_view, NRE.e_binder_view)
+let e_binders         : dualemb binders            = (RE.e_binders, NRE.e_binders)
+
+let e_letbinding      : dualemb letbinding         = (RE.e_letbinding, NRE.e_letbinding)
+let e_lb_view         : dualemb RD.lb_view         = (RE.e_lb_view, NRE.e_lb_view)
+(* ^ Inconsistent naming with these.. but too long otherwise, and userspace has
+ * lb_view already. Probably not worth the fix. *)
+
+let e_env             : dualemb Env.env            = (RE.e_env, NRE.e_env)
+let e_aqualv          : dualemb RD.aqualv          = (RE.e_aqualv, NRE.e_aqualv)
+let e_vconfig         : dualemb VConfig.vconfig    = (EMB.e_vconfig, NBET.e_vconfig)
+let e_attributes      : dualemb (list attribute)   = (RE.e_attributes, NRE.e_attributes)
+let e_qualifiers      : dualemb RD.qualifiers      = (RE.e_qualifiers, NRE.e_qualifiers)
+let e_range           : dualemb Range.range              =
+  (FStar.Syntax.Embeddings.e_range, FStar.TypeChecker.NBETerm.e_range)
+
+let nbe_dummy #a : NBET.embedding a =
+  let open FStar.Compiler.Effect in
+  NBET.mk_emb
+    (fun _ _ -> failwith "nbe_dummy embed")
+    (fun _ _ -> failwith "nbe_dummy unembed")
+    (NBET.mk_t NBET.Unknown)
+    ET_abstract
+
+let e_ident           : dualemb Ident.ident            = (RE.e_ident, nbe_dummy #Ident.ident)
+
+let e_subst           : dualemb (list subst_elt)   = (RE.e_subst, NRE.e_subst)
+
+let e_list (e : dualemb 'a) : dualemb (list 'a) =
+  (EMB.e_list (fst e), NBET.e_list (snd e))
+
+let e_option (e : dualemb 'a) : dualemb (option 'a) =
+  (EMB.e_option (fst e), NBET.e_option (snd e))
+
+let e_tuple2 (ea : dualemb 'a) (eb : dualemb 'b) : dualemb ('a & 'b) =
+  (EMB.e_tuple2 (fst ea) (fst eb), NBET.e_tuple2 (snd ea) (snd eb))
+
+let e_string_list = e_list e_string
+
+(** Helpers to create a (total) primitive step from a function and embeddings. *)
+let mk1' nm (f  : 'a  -> 'r) (ea  : dualemb 'a)
+        (er  : dualemb 'r): Cfg.primitive_step =
+    let l = mklid nm in
+    mk_us l 1 1 (int1     l f (fst ea) (fst er))
+           (nbe_int1 l f (snd ea) (snd er))
+
+let mk1 nm (f  : 'a  -> 'r) (ea  : dualemb 'a)
+        (er  : dualemb 'r): Cfg.primitive_step =
+    let l = mklid nm in
+    mk l 1 (int1     l f (fst ea) (fst er))
+           (nbe_int1 l f (snd ea) (snd er))
+
+let mk2 nm (f  : 'a  -> 'b -> 'r) (ea  : dualemb 'a) (eb : dualemb 'b)
+        (er  : dualemb 'r): Cfg.primitive_step =
+    let l = mklid nm in
+    mk l 2 (int2     l f (fst ea) (fst eb) (fst er))
+           (nbe_int2 l f (snd ea) (snd eb) (snd er))
+
+let mk3 nm (f  : 'a  -> 'b -> 'c -> 'r) (ea  : dualemb 'a) (eb : dualemb 'b) (ec : dualemb 'c)
+        (er  : dualemb 'r): Cfg.primitive_step =
+    let l = mklid nm in
+    mk l 3 (int3     l f (fst ea) (fst eb) (fst ec) (fst er))
+           (nbe_int3 l f (snd ea) (snd eb) (snd ec) (snd er))
+
+(*
+ * NOTE: all primitives must be carefully inspected to make sure they
+ * do not break the abstraction barrier imposed by the term_view.
+ * Otherwise, the pack_inspect_inv and inspect_pack_inv lemmas could
+ * likely be used to derive a contradiction.
+ *
+ * The way to go about adding new primitives is to implement them in the
+ * FStar.Reflection.V2.Builtins module and implement them using the (internal)
+ * inspect_ln and pack_ln functions, which means they should not break
+ * the view abstraction.
+ *
+ * _Any_ call to functions elsewhere, say term_to_string or
+ * Util.term_eq, will _very likely_ be inconsistent with the view.
+ * Exceptions to the "way to go" above should be well justified.
+ *)
+let reflection_primops : list Cfg.primitive_step = [
+  (****** Inspecting/packing various kinds of syntax ******)
+  mk1 "inspect_ln"
+    RB.inspect_ln
+    e_term
+    e_term_view;
+
+  mk1 "pack_ln"
+    RB.pack_ln
+    e_term_view
+    e_term;
+
+  mk1 "inspect_fv"
+    RB.inspect_fv
+    e_fv
+    e_string_list;
+
+  mk1 "pack_fv"
+    RB.pack_fv
+    e_string_list
+    e_fv;
+
+  mk1 "inspect_comp"
+    RB.inspect_comp
+    e_comp
+    e_comp_view;
+
+  mk1 "pack_comp"
+    RB.pack_comp
+    e_comp_view
+    e_comp;
+
+  mk1 "inspect_universe"
+    RB.inspect_universe
+    e_universe
+    e_universe_view;
+
+  mk1 "pack_universe"
+    RB.pack_universe
+    e_universe_view
+    e_universe;
+
+  mk1 "inspect_sigelt"
+    RB.inspect_sigelt
+    e_sigelt
+    e_sigelt_view;
+
+  mk1 "pack_sigelt"
+    RB.pack_sigelt
+    e_sigelt_view
+    e_sigelt;
+
+  mk1 "inspect_lb"
+    RB.inspect_lb
+    e_letbinding
+    e_lb_view;
+
+  mk1 "pack_lb"
+    RB.pack_lb
+    e_lb_view
+    e_letbinding;
+
+  mk1 "inspect_namedv"
+    RB.inspect_namedv
+    e_namedv
+    e_namedv_view;
+
+  mk1 "pack_namedv"
+    RB.pack_namedv
+    e_namedv_view
+    e_namedv;
+
+  mk1 "inspect_bv"
+    RB.inspect_bv
+    e_bv
+    e_bv_view;
+
+  mk1 "pack_bv"
+    RB.pack_bv
+    e_bv_view
+    e_bv;
+
+  (* TODO: Make this consistent with others? No good reason for it to be "exploded" *)
+  mk1 "inspect_binder"
+    RB.inspect_binder
+    e_binder
+    e_binder_view;
+
+  mk1 "pack_binder"
+    RB.pack_binder
+    e_binder_view
+    e_binder;
+
+  (****** Actual primitives ******)
+
+  mk1 "sigelt_opts"
+    RB.sigelt_opts
+    e_sigelt
+    (e_option e_vconfig);
+
+  (* This exposes the embedding of vconfig since it is useful to create attributes *)
+  mk1 "embed_vconfig"
+    RB.embed_vconfig
+    e_vconfig
+    e_term;
+
+  mk1 "sigelt_attrs"
+    RB.sigelt_attrs
+    e_sigelt
+    e_attributes;
+
+  mk2 "set_sigelt_attrs"
+    RB.set_sigelt_attrs
+    e_attributes  e_sigelt
+    e_sigelt;
+
+  mk1 "sigelt_quals"
+    RB.sigelt_quals
+    e_sigelt
+    e_qualifiers;
+
+  mk2 "set_sigelt_quals"
+    RB.set_sigelt_quals
+    e_qualifiers e_sigelt
+    e_sigelt;
+
+  mk2 "subst_term"
+    RB.subst_term
+    e_subst e_term e_term;
+
+  mk2 "subst_comp"
+    RB.subst_comp
+    e_subst e_comp e_comp;
+
+  mk2 "compare_bv"
+    RB.compare_bv
+    e_bv
+    e_bv
+    e_order;
+
+  mk2 "compare_namedv"
+    RB.compare_namedv
+    e_namedv
+    e_namedv
+    e_order;
+
+  mk2 "lookup_attr"
+    RB.lookup_attr
+    e_term
+    e_env
+    (e_list e_fv);
+
+  mk1 "all_defs_in_env"
+    RB.all_defs_in_env
+    e_env
+    (e_list e_fv);
+
+  mk2 "defs_in_module"
+    RB.defs_in_module
+    e_env
+    e_string_list
+    (e_list e_fv);
+
+  mk2 "term_eq"
+    RB.term_eq
+    e_term e_term
+    e_bool;
+
+  mk1 "moduleof"
+    RB.moduleof
+    e_env
+    e_string_list;
+
+  mk1 "vars_of_env"
+    RB.vars_of_env
+    e_env
+    (e_list e_binding);
+
+  mk2 "lookup_typ"
+    RB.lookup_typ
+    e_env
+    e_string_list
+    (e_option e_sigelt);
+
+  mk1 "env_open_modules"
+    RB.env_open_modules
+    e_env
+    (e_list e_string_list);
+
+  (* See note in ulib/FStar.Reflection.V2.Builints.fsti: we expose these
+     three to reduce dependencies. *)
+  mk1 "implode_qn"
+    RB.implode_qn
+    e_string_list
+    e_string;
+
+  mk1 "explode_qn"
+    RB.explode_qn
+    e_string
+    e_string_list;
+
+  mk2 "compare_string"
+    RB.compare_string
+    e_string e_string
+    e_int;
+
+  mk2 "push_namedv"
+    RB.push_namedv
+    e_env
+    e_namedv
+    e_env;
+
+  mk1 "range_of_term"
+    RB.range_of_term
+    e_term
+    e_range;
+
+  mk1 "range_of_sigelt"
+    RB.range_of_sigelt
+    e_sigelt
+    e_range;
+
+  mk1 "inspect_ident"
+    RB.inspect_ident
+    e_ident
+    (e_tuple2 e_string e_range);
+
+  mk1 "pack_ident"
+    RB.pack_ident
+    (e_tuple2 e_string e_range)
+    e_ident;
+]
+
+let _ = List.iter FStar.TypeChecker.Cfg.register_extra_step reflection_primops
