src/tactics/FStar.Tactics.Types.fst
@@ -110,3 +110,8 @@ let get_phi (g:goal) : option term =
 
 let is_irrelevant (g:goal) : bool =
     Option.isSome (get_phi g)
+
+let subtyping_token (g:env) (t0 t1:typ) = unit
+let equiv_token (g:env) (t0 t1:typ) = unit
+let typing_token (g:env) (e:term) (c:tot_or_ghost & typ) = unit
+let issues = list FStar.Issue.issue
