ulib/FStar.Tactics.NamedView.fst
@@ -1,0 +1,845 @@
+(*
+   Copyright 2008-2018 Microsoft Research
+
+   Licensed under the Apache License, Version 2.0 (the "License");
+   you may not use this file except in compliance with the License.
+   You may obtain a copy of the License at
+
+       http://www.apache.org/licenses/LICENSE-2.0
+
+   Unless required by applicable law or agreed to in writing, software
+   distributed under the License is distributed on an "AS IS" BASIS,
+   WITHOUT WARRANTIES OR CONDITIONS OF ANY KIND, either express or implied.
+   See the License for the specific language governing permissions and
+   limitations under the License.
+*)
+module FStar.Tactics.NamedView
+
+(* inner let bindings not encoded, OK *)
+#set-options "--warn_error -242"
+
+(* This file is part of the tactics core, we open only what's needed. *)
+open FStar.Tactics.Effect
+open FStar.Tactics.Util
+open FStar.Tactics.V2.Builtins
+
+exception LengthMismatch
+exception NotEnoughBinders
+
+(* We work with reflection V2. *)
+open FStar.Reflection.V2
+module R = FStar.Reflection.V2
+module RD = FStar.Reflection.V2.Data
+
+(* Disable printing, but mark private so we don't mess
+with clients. *)
+private
+let print (s:string) : Tac unit = ()
+
+(* Re export the syntax types. Expose variables as their views, users do
+not need to pack/inspect these if they are using the named view. *)
+let namedv   = R.namedv_view
+let bv       = R.bv_view
+let comp     = R.comp_view
+let binding  = R.binding (* already good *)
+(* Terms and universes are still *deep*, so we do not change their
+representation, and the user needs to pack/inspect. *)
+let term     = R.term
+let universe = R.universe
+
+[@@plugin]
+noeq
+type binder = {
+  uniq   : nat;
+
+  ppname : ppname_t;
+  sort   : typ;
+  qual   : aqualv;
+  attrs  : list term;
+}
+type binders = list binder
+
+let is_simple_binder (b:binder) = Q_Explicit? b.qual /\ Nil? b.attrs
+type simple_binder = b:binder{is_simple_binder b}
+
+type univ_name = string & Range.range
+
+[@@plugin]
+noeq
+type universe_view =
+  | Uv_Zero : universe_view
+  | Uv_Succ : universe -> universe_view
+  | Uv_Max  : universes -> universe_view
+  | Uv_BVar : nat -> universe_view
+  | Uv_Name : univ_name -> universe_view
+  | Uv_Unif : universe_uvar -> universe_view
+  | Uv_Unk  : universe_view
+
+[@@plugin]
+noeq
+type pattern =
+ // A built-in constant
+ | Pat_Constant {
+     c : vconst
+   }
+
+ // A fully applied constructor, each boolean marks whether the
+ // argument was an explicitly-provided implicit argument
+ | Pat_Cons {
+     head    : fv;
+     univs   : option universes;
+     subpats : list (pattern * bool)
+   }
+
+ // A pattern-bound *named* variable.
+ | Pat_Var {
+     v    : namedv;
+     sort : sealed typ;
+   }
+
+ // Dot pattern: resolved by other elements in the pattern and type
+ | Pat_Dot_Term {
+     t : option term;
+   }
+
+type branch = pattern & term
+type match_returns_ascription = binder & (either term comp & option term & bool)
+
+[@@plugin]
+noeq
+type named_term_view =
+  | Tv_Var    : v:namedv -> named_term_view
+  | Tv_BVar   : v:bv -> named_term_view
+  | Tv_FVar   : v:fv -> named_term_view
+  | Tv_UInst  : v:fv -> us:universes -> named_term_view
+  | Tv_App    : hd:term -> a:argv -> named_term_view
+  | Tv_Abs    : bv:binder -> body:term -> named_term_view
+  | Tv_Arrow  : bv:binder -> c:comp -> named_term_view
+  | Tv_Type   : universe -> named_term_view
+  | Tv_Refine : b:simple_binder -> ref:term -> named_term_view
+  | Tv_Const  : vconst -> named_term_view
+  | Tv_Uvar   : nat -> ctx_uvar_and_subst -> named_term_view
+  | Tv_Let    : recf:bool -> attrs:(list term) -> b:simple_binder -> def:term -> body:term -> named_term_view
+  | Tv_Match  : scrutinee:term -> ret:option match_returns_ascription -> brs:(list branch) -> named_term_view
+  | Tv_AscribedT : e:term -> t:term -> tac:option term -> use_eq:bool -> named_term_view
+  | Tv_AscribedC : e:term -> c:comp -> tac:option term -> use_eq:bool -> named_term_view
+  | Tv_Unknown  : named_term_view // An underscore: _
+  | Tv_Unsupp : named_term_view // failed to inspect, not supported
+
+private
+let __binding_to_binder (bnd : binding) (b : R.binder) : binder =
+  {
+      ppname = bnd.ppname;
+      uniq   = bnd.uniq;
+      sort   = bnd.sort;
+      qual   = (inspect_binder b).qual;
+      attrs  = (inspect_binder b).attrs;
+  }
+
+let binding_to_binder (bnd : binding) : binder =
+  {
+      ppname = bnd.ppname;
+      uniq   = bnd.uniq;
+      sort   = bnd.sort;
+      qual   = Q_Explicit;
+      attrs  = []
+  }
+
+let binder_to_binding (b : binder) : binding =
+  {
+      ppname = b.ppname;
+      uniq   = b.uniq;
+      sort   = b.sort;
+  }
+
+private
+let r_binder_to_namedv (b : binder) : R.namedv =
+  pack_namedv {
+    uniq   = b.uniq;
+    sort   = seal b.sort;
+    ppname = b.ppname;
+  }
+
+let namedv_to_binder (v : namedv) (sort : term) : binder =
+  {
+    uniq   = v.uniq;
+    sort   = sort;
+    ppname = v.ppname;
+    qual   = Q_Explicit;
+    attrs  = [];
+  }
+
+(* Bindings and simple_binders are the same *)
+let binding_to_simple_binder (b:binding) : simple_binder = {
+  uniq   = b.uniq;
+  sort   = b.sort;
+  ppname = b.ppname;
+  qual   = Q_Explicit;
+  attrs  = [];
+}
+let simple_binder_to_binding (b:simple_binder) : binding = {
+  uniq   = b.uniq;
+  sort   = b.sort;
+  ppname = b.ppname;
+}
+
+let open_universe_view (v:RD.universe_view) : universe_view =
+  match v with
+  | R.Uv_Zero -> Uv_Zero
+  | R.Uv_Succ u -> Uv_Succ u
+  | R.Uv_Max us -> Uv_Max us
+  | R.Uv_BVar n -> Uv_BVar n
+  | R.Uv_Name i -> Uv_Name (inspect_ident i)
+  | R.Uv_Unif uvar -> Uv_Unif uvar
+  | R.Uv_Unk -> Uv_Unk
+
+let inspect_universe (u:universe) : universe_view =
+  let v = R.inspect_universe u in
+  open_universe_view v
+
+let close_universe_view (v:universe_view) : R.universe_view =
+  match v with
+  | Uv_Zero -> R.Uv_Zero
+  | Uv_Succ u -> R.Uv_Succ u
+  | Uv_Max us -> R.Uv_Max us
+  | Uv_BVar n -> R.Uv_BVar n
+  | Uv_Name i -> R.Uv_Name (pack_ident i)
+  | Uv_Unif uvar -> R.Uv_Unif uvar
+  | Uv_Unk -> R.Uv_Unk
+
+let pack_universe (uv:universe_view) : universe =
+  let uv = close_universe_view uv in
+  R.pack_universe uv
+
+private
+let open_binder (b : R.binder) : Tac binder =
+  let n = fresh () in
+  let bv = inspect_binder b in
+  {
+    uniq   = n;
+    sort   = bv.sort;
+    ppname = bv.ppname;
+    qual   = bv.qual;
+    attrs  = bv.attrs;
+  }
+
+private
+let close_binder (b : binder) : R.binder =
+  pack_binder {
+    sort   = b.sort;
+    qual   = b.qual;
+    ppname = b.ppname;
+    attrs  = b.attrs;
+  }
+
+private
+let open_term_with (b : R.binder) (nb : binder) (t : term) : Tac term =
+  let nv : R.namedv = pack_namedv {
+    uniq   = nb.uniq;
+    sort   = seal nb.sort;
+    ppname = nb.ppname;
+  }
+  in
+  let t' = subst_term [DB 0 nv] t in
+  t'
+
+private
+let open_term (b : R.binder) (t : term) : Tac (binder & term) =
+  let bndr : binder = open_binder b in
+  (bndr, open_term_with b bndr t)
+
+let subst_comp (s : subst_t) (c : comp) : comp =
+  inspect_comp (R.subst_comp s (pack_comp c))
+
+private
+let open_comp (b : R.binder) (t : comp) : Tac (binder & comp) =
+  let n = fresh () in
+  let bv : binder_view = inspect_binder b in
+  let nv : R.namedv = pack_namedv {
+    uniq   = n;
+    sort   = seal bv.sort;
+    ppname = bv.ppname;
+  }
+  in
+  let t' = subst_comp [DB 0 nv] t in
+  let bndr : binder = {
+    uniq   = n;
+    sort   = bv.sort;
+    ppname = bv.ppname;
+    qual   = bv.qual;
+    attrs  = bv.attrs;
+  }
+  in
+  (bndr, t')
+
+private
+let open_comp_with (b : R.binder) (nb : binder) (c : comp) : Tac comp =
+  let nv : R.namedv = pack_namedv {
+    uniq   = nb.uniq;
+    sort   = seal nb.sort;
+    ppname = nb.ppname;
+  }
+  in
+  let t' = subst_comp [DB 0 nv] c in
+  t'
+
+(* FIXME: unfortunate duplication here. The effect means this proof cannot
+be done extrinsically. Can we add a refinement to the binder? *)
+private
+let open_term_simple (b : R.simple_binder) (t : term) : Tac (simple_binder & term) =
+  let n = fresh () in
+  let bv : binder_view = inspect_binder b in
+  let nv : R.namedv = pack_namedv {
+    uniq   = n;
+    sort   = seal bv.sort;
+    ppname = bv.ppname;
+  }
+  in
+  let t' = subst_term [DB 0 nv] t in
+  let bndr : binder = {
+    uniq   = n;
+    sort   = bv.sort;
+    ppname = bv.ppname;
+    qual   = bv.qual;
+    attrs  = bv.attrs;
+  }
+  in
+  (bndr, t')
+
+private
+let open_comp_simple (b : R.simple_binder) (t : comp) : Tac (simple_binder & comp) =
+  let n = fresh () in
+  let bv : binder_view = inspect_binder b in
+  let nv : R.namedv = pack_namedv {
+    uniq   = n;
+    sort   = seal bv.sort;
+    ppname = bv.ppname;
+  }
+  in
+  let t' = subst_comp [DB 0 nv] t in
+  let bndr : binder = {
+    uniq   = n;
+    sort   = bv.sort;
+    ppname = bv.ppname;
+    qual   = bv.qual;
+    attrs  = bv.attrs;
+  }
+  in
+  (bndr, t')
+
+(* This can be useful externally *)
+let close_term (b:binder) (t:term) : R.binder & term =
+  let nv = r_binder_to_namedv b in
+  let t' = subst_term [NM nv 0] t in
+  let b = pack_binder { sort = b.sort; ppname = b.ppname; qual = b.qual; attrs = b.attrs } in
+  (b, t')
+private
+let close_comp (b:binder) (t:comp) : R.binder & comp =
+  let nv = r_binder_to_namedv b in
+  let t' = subst_comp [NM nv 0] t in
+  let b = pack_binder { sort = b.sort; ppname = b.ppname; qual = b.qual; attrs = b.attrs } in
+  (b, t')
+
+private
+let close_term_simple (b:simple_binder) (t:term) : R.simple_binder & term =
+  let nv = r_binder_to_namedv b in
+  let t' = subst_term [NM nv 0] t in
+  let bv : binder_view = { sort = b.sort; ppname = b.ppname; qual = b.qual; attrs = b.attrs } in
+  let b = pack_binder bv in
+  inspect_pack_binder bv;
+  (b, t')
+private
+let close_comp_simple (b:simple_binder) (t:comp) : R.simple_binder & comp =
+  let nv = r_binder_to_namedv b in
+  let t' = subst_comp [NM nv 0] t in
+  let bv : binder_view = { sort = b.sort; ppname = b.ppname; qual = b.qual; attrs = b.attrs } in
+  let b = pack_binder bv in
+  inspect_pack_binder bv;
+  (b, t')
+
+private
+let r_subst_binder_sort (s : subst_t) (b : R.binder) : R.binder =
+  let v = inspect_binder b in
+  let v = { v with sort = subst_term s v.sort } in
+  pack_binder v
+
+let subst_binder_sort (s : subst_t) (b : binder) : binder =
+  { b with sort = subst_term s b.sort }
+
+(* Can't define this inside open_term_n. See #2955 *)
+private
+let rec __open_term_n_aux (bs : list R.binder) (nbs : list binder) (s : subst_t) : Tac (list binder & subst_t) =
+  match bs with
+  | [] -> nbs, s
+  | b::bs ->
+    let b = r_subst_binder_sort s b in
+    let b = open_binder b in
+    let nv = r_binder_to_namedv b in
+    __open_term_n_aux bs (b::nbs) (DB 0 nv :: shift_subst 1 s)
+
+private
+let open_term_n (bs : list R.binder) (t : term) : Tac (list binder & term) =
+  let nbs, s = __open_term_n_aux bs [] [] in
+  List.Tot.rev nbs, subst_term s t
+
+private
+let rec open_term_n_with (bs : list R.binder) (nbs : list binder) (t : term) : Tac term =
+  match bs, nbs with
+  | [], [] -> t
+  | b::bs, nb::nbs ->
+    let t' = open_term_n_with bs nbs t in
+    let t'' = open_term_with b nb t' in
+    t''
+  | _ -> raise LengthMismatch
+
+private
+let close_term_n (bs : list binder) (t : term) : list R.binder & term =
+  let rec aux (bs : list binder) (cbs : list R.binder) (s : subst_t) : list R.binder & subst_t =
+    match bs with
+    | [] -> cbs, s
+    | b::bs ->
+      let b = subst_binder_sort s b in
+      let nv = r_binder_to_namedv b in
+      let b = close_binder b in
+      aux bs (b::cbs) (NM nv 0 :: shift_subst 1 s)
+  in
+  let cbs, s = aux bs [] [] in
+  List.Tot.rev cbs, subst_term s t
+
+private
+let rec open_term_n_simple (bs : list R.simple_binder) (t : term) : Tac (list simple_binder & term) =
+  match bs with
+  | [] -> ([], t)
+  | b::bs ->
+    let bs', t' = open_term_n_simple bs t in
+    let b', t'' = open_term_simple b t' in
+    (b'::bs', t'')
+
+private
+let rec close_term_n_simple (bs : list simple_binder) (t : term) : list R.simple_binder & term =
+  match bs with
+  | [] -> ([], t)
+  | b::bs ->
+    let bs', t' = close_term_n_simple bs t in
+    let b', t'' = close_term_simple b t' in
+    (b'::bs', t'')
+
+private
+let rec open_pat (p : R.pattern) (s : subst_t) : Tac (pattern & subst_t) =
+  match p with
+  | R.Pat_Constant c ->
+    Pat_Constant {c=c}, s
+
+  | R.Pat_Var ssort n ->
+    let sort = unseal ssort in
+    let sort = subst_term s sort in
+    let nvv : namedv = {
+      uniq = fresh();
+      sort = seal sort;
+      ppname = n;
+    }
+    in
+    let nv = pack_namedv nvv in
+    Pat_Var {v=nvv; sort=seal sort}, (DB 0 nv) :: shift_subst 1 s
+
+  | R.Pat_Cons head univs subpats ->
+    let subpats, s = fold_left (fun (pats,s) (pat,b) ->
+                        let pat, s' = open_pat pat s in
+                        ((pat,b)::pats, s'))
+                       ([], s) subpats
+    in
+    let subpats = List.Tot.rev subpats in
+    Pat_Cons {head=head; univs=univs; subpats=subpats}, s
+
+  | R.Pat_Dot_Term None ->
+    Pat_Dot_Term {t=None}, s
+
+  | R.Pat_Dot_Term (Some t) ->
+    let t = subst_term s t in
+    Pat_Dot_Term {t=Some t}, s
+
+private
+let open_branch (b : R.branch) : Tac branch =
+  let (pat, t) = b in
+  let pat, s = open_pat pat [] in
+  let t' = subst_term s t in
+  (pat, t')
+
+private
+let rec close_pat (p : pattern) (s : subst_t) : Tot (R.pattern & subst_t) =
+  match p with
+  | Pat_Constant {c} ->
+    R.Pat_Constant c, s
+
+  | Pat_Var {v; sort} ->
+    let nv = pack_namedv v in
+    (* NOTE: we cannot do anything on the sort wihtout going
+    into TAC. Need a sealed_bind. *)
+    //let sort = unseal sort in
+    //let sort = subst_term s sort in
+    //let sort = seal sort in
+    let s = (NM nv 0) :: shift_subst 1 s in
+    R.Pat_Var sort v.ppname, s
+
+  | Pat_Cons {head; univs; subpats} ->
+    let subpats, s = List.Tot.fold_left (fun (pats,s) (pat,b) ->
+                        assume(pat << p);
+                        let pat, s' = close_pat pat s in
+                        ((pat,b)::pats, s'))
+                       ([], s) subpats
+    in
+    let subpats = List.Tot.rev subpats in
+    R.Pat_Cons head univs subpats, s
+
+  | Pat_Dot_Term {t=None} ->
+    R.Pat_Dot_Term None, s
+
+  | Pat_Dot_Term {t=Some t} ->
+    let t = subst_term s t in
+    R.Pat_Dot_Term (Some t), s
+
+private
+let close_branch (b : branch) : Tot R.branch =
+  let (pat, t) = b in
+  let pat, s = close_pat pat [] in
+  let t' = subst_term s t in
+  (pat, t')
+
+private
+let open_match_returns_ascription (mra : R.match_returns_ascription) : Tac match_returns_ascription =
+  let (b, (ct, topt, use_eq)) = mra in
+  let nb = open_binder b in
+  let ct = match ct with
+    | Inl t -> Inl (open_term_with b nb t)
+    | Inr c ->
+      let c = inspect_comp c in
+      let c = open_comp_with b nb c in
+      Inr c
+  in
+  let topt =
+    match topt with
+    | None -> None
+    | Some t -> Some (open_term_with b nb t)
+  in
+  (nb, (ct, topt, use_eq))
+
+private
+let close_match_returns_ascription (mra : match_returns_ascription) : R.match_returns_ascription =
+  let (nb, (ct, topt, use_eq)) = mra in
+  let b = close_binder nb in
+  // FIXME: all this is repeating the close_binder work, for no good reason
+  let ct = match ct with
+    | Inl t -> Inl (snd (close_term nb t))
+    | Inr c ->
+      let _, c = close_comp nb c in
+      let c = pack_comp c in
+      Inr c
+  in
+  let topt =
+    match topt with
+    | None -> None
+    | Some t -> Some (snd (close_term nb t))
+  in
+  (b, (ct, topt, use_eq))
+
+private
+let open_view (tv:term_view) : Tac named_term_view =
+  match tv with
+  (* Nothing interesting *)
+  | RD.Tv_Var v -> Tv_Var (inspect_namedv v)
+  | RD.Tv_BVar v -> Tv_BVar (inspect_bv v)
+  | RD.Tv_FVar v -> Tv_FVar v
+  | RD.Tv_UInst v us -> Tv_UInst v us
+  | RD.Tv_App hd a -> Tv_App hd a
+  | RD.Tv_Type u -> Tv_Type u
+  | RD.Tv_Const c -> Tv_Const c
+  | RD.Tv_Uvar n ctx_uvar_and_subst -> Tv_Uvar n ctx_uvar_and_subst
+  | RD.Tv_AscribedT e t tac use_eq -> Tv_AscribedT e t tac use_eq
+  | RD.Tv_AscribedC e c tac use_eq -> Tv_AscribedC e (inspect_comp c) tac use_eq
+  | RD.Tv_Unknown -> Tv_Unknown
+  | RD.Tv_Unsupp -> Tv_Unsupp
+
+  (* Below are the nodes that actually involve a binder.
+  Open them and convert to named binders. *)
+
+  | RD.Tv_Abs b body ->
+    let nb, body = open_term b body in
+    Tv_Abs nb body
+
+  | RD.Tv_Arrow b c ->
+    let nb, c = open_comp b (inspect_comp c) in
+    Tv_Arrow nb c
+
+  | RD.Tv_Refine b ref ->
+    let nb, ref = open_term_simple b ref in
+    Tv_Refine nb ref
+
+  | RD.Tv_Let recf attrs b def body ->
+    let nb, body = open_term_simple b body in
+    let def =
+      if recf
+      then subst_term [DB 0 (r_binder_to_namedv nb)] def
+      else def
+    in
+    Tv_Let recf attrs nb def body
+
+  | RD.Tv_Match scrutinee ret brs ->
+    let brs = map open_branch brs in
+    let ret = map_opt open_match_returns_ascription ret in
+    Tv_Match scrutinee ret brs
+
+private
+let close_view (tv : named_term_view) : Tot term_view =
+  match tv with
+  (* Nothing interesting *)
+  | Tv_Var v -> RD.Tv_Var (pack_namedv v)
+  | Tv_BVar v -> RD.Tv_BVar (pack_bv v)
+  | Tv_FVar v -> RD.Tv_FVar v
+  | Tv_UInst v us -> RD.Tv_UInst v us
+  | Tv_App hd a -> RD.Tv_App hd a
+  | Tv_Type u -> RD.Tv_Type u 
+  | Tv_Const c -> RD.Tv_Const c
+  | Tv_Uvar n ctx_uvar_and_subst -> RD.Tv_Uvar n ctx_uvar_and_subst
+  | Tv_AscribedT e t tac use_eq -> RD.Tv_AscribedT e t tac use_eq
+  | Tv_AscribedC e c tac use_eq -> RD.Tv_AscribedC e (pack_comp c) tac use_eq
+  | Tv_Unknown -> RD.Tv_Unknown
+  | Tv_Unsupp -> RD.Tv_Unsupp
+
+  (* Below are the nodes that actually involve a binder.
+  Open them and convert to named binders. *)
+
+  | Tv_Abs nb body ->
+    let b, body = close_term nb body in
+    RD.Tv_Abs b body
+
+  | Tv_Arrow nb c ->
+    let b, c = close_comp nb c in
+    let c = pack_comp c in
+    RD.Tv_Arrow b c
+
+  | Tv_Refine nb ref ->
+    let b, ref = close_term_simple nb ref in
+    RD.Tv_Refine b ref
+
+  | Tv_Let recf attrs nb def body ->
+    let def =
+      if recf
+      then subst_term [NM (r_binder_to_namedv nb) 0] def
+      else def
+    in
+    let b, body = close_term_simple nb body in
+    RD.Tv_Let recf attrs b def body
+
+  | Tv_Match scrutinee ret brs ->
+    let brs = List.Tot.map close_branch brs in
+    let ret = FStar.Option.mapTot close_match_returns_ascription ret in
+    RD.Tv_Match scrutinee ret brs
+
+[@@plugin]
+let inspect (t:term) : Tac named_term_view =
+  let t = compress t in
+  let tv = inspect_ln t in
+  open_view tv
+
+[@@plugin]
+let pack (tv:named_term_view) : Tot term =
+  let tv = close_view tv in
+  pack_ln tv
+
+// Repeat from FStar.R.Data
+let notAscription (tv:named_term_view) : bool =
+  not (Tv_AscribedT? tv) && not (Tv_AscribedC? tv)
+
+[@@plugin]
+noeq
+type letbinding = {
+  lb_fv : fv;
+  lb_us : list univ_name; (* opened *)
+  lb_typ : typ;
+  lb_def : term;
+}
+
+[@@plugin]
+noeq
+type named_sigelt_view =
+  | Sg_Let {
+      isrec : bool;
+      lbs   : list letbinding;
+    }
+
+  // Sg_Inductive basically coalesces the Sig_bundle used internally,
+  // where the type definition and its constructors are split.
+  // While that might be better for typechecking, this is probably better for metaprogrammers
+  // (no mutually defined types for now)
+  | Sg_Inductive {
+      nm     : name;             // name of the inductive type being defined
+      univs  : list univ_name;   // named universe variables
+      params : binders;          // parameters
+      typ    : typ;              // the type annotation for the inductive, i.e., indices -> Type #u
+      ctors  : list ctor;        // the constructors, opened with univs and applied to params already
+    }
+
+  | Sg_Val {
+      nm    : name;
+      univs : list univ_name;
+      typ   : typ;
+    }
+
+  | Unk
+
+private
+let open_univ_s (us : list R.univ_name) : Tac (list univ_name & subst_t) =
+  let n = List.Tot.length us in
+  let s = mapi (fun i u -> UN (n-1-i) (R.pack_universe (R.Uv_Name u))) us in
+  Util.map (fun i -> inspect_ident i) us, s
+
+private
+let close_univ_s (us : list univ_name) : list R.univ_name & subst_t =
+  let n = List.Tot.length us in
+  let us = List.Tot.map (fun i -> pack_ident i) us in
+  let s = List.Tot.mapi (fun i u -> UD u (n-i-1)) us in
+  us, s
+
+private
+let open_lb (lb : R.letbinding) : Tac letbinding =
+  let {lb_fv; lb_us; lb_typ; lb_def} = inspect_lb lb in
+  let lb_us, s = open_univ_s lb_us in
+  let lb_typ = subst_term s lb_typ in
+  let lb_def = subst_term s lb_def in
+  { lb_fv; lb_us; lb_typ; lb_def }
+
+private
+let close_lb (lb : letbinding) : R.letbinding =
+  let {lb_fv; lb_us; lb_typ; lb_def} = lb in
+  let lb_us, s = close_univ_s lb_us in
+  let lb_typ = subst_term s lb_typ in
+  let lb_def = subst_term s lb_def in
+  pack_lb { lb_fv; lb_us; lb_typ; lb_def }
+
+private
+let subst_r_binders (s:subst_t) (bs : list R.binder) : list R.binder =
+  List.Tot.mapi (fun i b -> r_subst_binder_sort (shift_subst i s) b) bs
+
+private
+let rec open_n_binders_from_arrow (bs : binders) (t : term) : Tac term =
+  match bs with
+  | [] -> t
+  | b::bs ->
+    match inspect t with
+    | Tv_Arrow b' (C_Total t') ->
+      let t' = subst_term [NT (r_binder_to_namedv b') (pack (Tv_Var (inspect_namedv (r_binder_to_namedv b))))] t' in
+      open_n_binders_from_arrow bs t'
+    | _ -> raise NotEnoughBinders
+
+private
+let open_sigelt_view (sv : sigelt_view) : Tac named_sigelt_view =
+  match sv with
+  | RD.Sg_Let isrec lbs ->
+    let lbs = map open_lb lbs in
+    (* open universes, maybe *)
+    Sg_Let { isrec; lbs }
+
+  | RD.Sg_Inductive nm univs params typ ctors ->
+    let nparams = List.Tot.length params in
+
+    (* Open universes everywhere *)
+    let univs, s = open_univ_s univs in
+    let params = subst_r_binders s params in
+    let typ = subst_term (shift_subst nparams s) typ in
+    let ctors = map (fun (nm, ty) -> nm, subst_term s ty) ctors in
+
+    (* Open parameters in themselves and in type *)
+    let params, typ = open_term_n params typ in
+    (* Remove the parameter binders from the constructors,
+    replace them by the opened param binders. Hence we get
+      Cons : a0 -> list a0
+    instead of
+      Cons : #a:Type -> a -> list a
+    for the returned open parameter a0. *)
+    let ctors =
+      map (fun (nm, ty) ->
+          let ty'= open_n_binders_from_arrow params ty in
+          nm, ty')
+        ctors
+    in
+
+    Sg_Inductive {nm; univs; params; typ; ctors}
+
+  | RD.Sg_Val nm univs typ ->
+    let univs, s = open_univ_s univs in
+    let typ = subst_term s typ in
+    Sg_Val {nm; univs; typ}
+
+  | RD.Unk -> Unk
+
+private
+let rec mk_arr (args : list binder) (t : term) : Tac term =
+  match args with
+  | [] -> t
+  | a :: args' ->
+    let t' = C_Total (mk_arr args' t) in
+    pack (Tv_Arrow a t')
+
+private
+let close_sigelt_view (sv : named_sigelt_view{~(Unk? sv)}) : Tac (sv:sigelt_view{~(RD.Unk? sv)}) =
+  match sv with
+  | Sg_Let { isrec; lbs } ->
+    let lbs = List.Tot.map close_lb lbs in
+    RD.Sg_Let isrec lbs
+
+  | Sg_Inductive {nm; univs; params; typ; ctors} ->
+    let nparams = List.Tot.length params in
+    (* Abstract constructors by the parameters. This
+    is the inverse of the open_n_binders_from_arrow above. *)
+    let ctors =
+        map (fun (nm, ty) ->
+            let ty' = mk_arr params ty in
+            nm, ty')
+        ctors
+    in
+
+    (* Close parameters in themselves and typ *)
+    let params, typ = close_term_n params typ in
+
+    (* close univs *)
+    let univs, s = close_univ_s univs in
+    let params = subst_r_binders s params in
+    let typ = subst_term (shift_subst nparams s) typ in
+    let ctors = map (fun (nm, ty) -> nm, subst_term s ty) ctors in
+
+    RD.Sg_Inductive nm univs params typ ctors
+
+  | Sg_Val {nm; univs; typ} ->
+    let univs, s = close_univ_s univs in
+    let typ = subst_term s typ in
+    RD.Sg_Val nm univs typ
+
+[@@plugin]
+let inspect_sigelt (s : sigelt) : Tac named_sigelt_view =
+  let sv = R.inspect_sigelt s in
+  (* dump ("sv orig = " ^ term_to_string (quote sv)); *)
+  open_sigelt_view sv
+
+[@@plugin]
+let pack_sigelt (sv:named_sigelt_view{~(Unk? sv)}) : Tac sigelt =
+  let sv = close_sigelt_view sv in
+  R.pack_sigelt sv
+
+(* Clients of this module use the named view. *)
+let term_view   = named_term_view
+let sigelt_view = named_sigelt_view
+
+(* Temporary adapters, to avoid breaking existing code too much. *)
+let inspect_namedv   = id #namedv
+let pack_namedv      = id #namedv
+let inspect_bv       = id #bv
+let pack_bv          = id #bv
+let inspect_comp     = id #comp
+let pack_comp        = id #comp
+
+(* Some primitives mention `comp`, wrap them to use `comp_view` *)
+let tcc (e:env) (t:term) : Tac comp =
+  let c : R.comp = V2.Builtins.tcc e t in
+  R.inspect_comp c
+
+let comp_to_string (c:comp) : Tac string = V2.Builtins.comp_to_string (R.pack_comp c)
